formal/inference/heuristics/Separation.thy
@@ -1,5 +1,0 @@
-theory Separation
-imports "../Inference"
-begin
-
-end
